verif/verif_entryindex.v
@@ -37,30 +37,30 @@ Qed.
 Lemma body_entryIndex: semax_body Vprog Gprog f_entryIndex entryIndex_spec.
 Proof.
   start_function.
-  destruct r as [[[root numRec] depth] prel].
-  pose (r:=(root,numRec,depth,prel)).
+  destruct r as [root prel].
+  pose (r:=(root,prel)).
   unfold cursor_rep. Intros anc_end. Intros Idx_end.
   forward.                      (* t'1=cursor->level *)
   destruct c as [|[n i ]c'].
-  - inv H; inv H0; inv H1. inv H0. (* no empty cursor *)
+  - inv H; inv H1; inv H2. inv H1. (* no empty cursor *)
   - forward.                      (* t'2=cursor->ancestorsIdx[t'1] *)
     + entailer!.
-      apply partial_complete_length in H. auto.
+      apply partial_complete_length in H. auto. auto.
     + entailer!. autorewrite with sublist.
       assert (Z.succ (Zlength c') -1 - Zlength c' = 0) by omega.
-      rewrite H7. unfold Znth. simpl.
+      rewrite H8. unfold Znth. simpl.
       unfold rep_index. destruct i; auto.
     + autorewrite with sublist. deadvars!.
       destruct r. autorewrite with norm.
-      assert(Z.succ (Zlength c') -1 = Zlength c') by omega. rewrite H0.
+      assert(Z.succ (Zlength c') -1 = Zlength c') by omega. rewrite H1.
       pose (c'':=map (fun x : node val * index.index => rep_index (snd x)) c'). fold c''.
       assert (Zlength c'' = Zlength c') by (unfold c''; rewrite Zlength_map; auto).
-      rewrite <- H1.
+      rewrite <- H2.
       rewrite Znth_rev_cons by auto.
       forward. cancel.
       unfold cursor_rep.
       Exists (anc_end). Exists (Idx_end). cancel.
-      rewrite H1. assert (Zlength ((n, i) :: c') - 1 = Zlength c').
-      rewrite Zlength_cons. omega. rewrite H10.
+      rewrite H2. assert (Zlength ((n, i) :: c') - 1 = Zlength c').
+      rewrite Zlength_cons. omega. rewrite H11.
       cancel.
 Qed.
