verif/verif_findindex.v
@@ -30,12 +30,14 @@ Proof.
   forward_if (PROP ( )
      LOCAL (temp _t'7 (Vint (Int.repr (Z.of_nat (numKeys (btnode val ptr0 le false First Last pn)))));
      temp _i (Vint (Int.repr 0)); temp _node (getval (btnode val ptr0 le false First Last pn));
-     temp _key (Vint (Int.repr key)))  SEP (btnode_rep n)).
+     temp _key (key_repr key))  SEP (btnode_rep n)).
   - forward.                    (* skip *)
     entailer!.
   - apply intern_le_cons in H0. destruct H0. destruct H0. rewrite H0 in H. simpl in H.
-    (* contradiction in H *)
-    admit. simpl. auto.
+    pose (num := numKeys_le x0). fold num in H. rewrite Zpos_P_of_succ_nat in H.
+    rewrite Int.signed_repr in H. omega.
+    split. rep_omega. unfold node_wf in H1. rewrite H0 in H1. simpl in H1. unfold num.
+    rep_omega. simpl. auto.
   - destruct le as [|e le'] eqn:HLE.
     { apply intern_le_cons in H0. destruct H0. destruct H. inv H. simpl. auto. }
     destruct e eqn:HE.
@@ -46,26 +48,27 @@ Proof.
     forward_if.
     + forward.                  (* return *)
       entailer!. unfold findChildIndex'. simpl.
-      assert (key <? k = true).
-      admit.                    (* true because of H *)
-      rewrite H5. Exists ent_end0. entailer!.
+      rewrite key_unsigned_repr in H. rewrite key_unsigned_repr in H.
+      apply Fcore_Zaux.Zlt_bool_true in H. rewrite H. simpl.
+      Exists ent_end0. entailer!.
     + forward.                  (* skip *)
       forward.                  (* i=0 *)
       gather_SEP 0 1 2 3 4 5. replace_SEP 0 (btnode_rep n). { entailer!. Exists ent_end0. entailer!. } deadvars!.
       
-{ forward_loop (EX i:Z, PROP(i<=idx_to_Z (findChildIndex n key)) LOCAL(temp _i (Vint(Int.repr i)); temp _node pn; temp _key (Vint(Int.repr key))) SEP(btnode_rep n))
-                   break:(EX i:Z, PROP(i=idx_to_Z (findChildIndex n key)) LOCAL(temp _i (Vint(Int.repr i)); temp _node pn; temp _key (Vint(Int.repr key))) SEP(btnode_rep n)).
+{ forward_loop (EX i:Z, PROP(i<=idx_to_Z (findChildIndex n key)) LOCAL(temp _i (Vint(Int.repr i)); temp _node pn; temp _key (key_repr key)) SEP(btnode_rep n))
+                   break:(EX i:Z, PROP(i=idx_to_Z (findChildIndex n key)) LOCAL(temp _i (Vint(Int.repr i)); temp _node pn; temp _key (key_repr key)) SEP(btnode_rep n)).
 
   - Exists 0. entailer!.
-    assert (key <? k = false). admit.   (* true from H *)
-    rewrite H1.
+    rewrite key_unsigned_repr in H. rewrite key_unsigned_repr in H.
+    assert (key.(k_) <? k.(k_) = false). admit.   (* true from H *)
+    rewrite H2.
     admit.                      (* OK because fCI' is called with ip 0 *)
   - Intros i.
     rewrite unfold_btnode_rep. unfold n. Intros ent_end1.
     forward.                    (* t'5=node->numKeys *)
     gather_SEP 0 1 2 3 4 5 6. replace_SEP 0 (btnode_rep n). { entailer!. Exists ent_end1. entailer!. } 
     assert((numKeys (btnode val ptr0 (cons val (keychild val k n0) le') false First Last pn)) = S (numKeys_le le')). simpl. auto.
-    rewrite H2.
+    rewrite H3.
     forward_if.
     + entailer!. admit.         (* le not to large *)
     + forward.                  (* skip *)
